SP1Clean/JalrChip.lean
@@ -15,9 +15,9 @@ import SP1Operations.Reader.ITypeReader.ITypeReader
 import SP1Chips.Jalr.JalrChip
 import SP1Chips.Jalr.Common
 import SP1Chips.Soundness
-import SP1Clean.AddOperation
+import SP1Clean.Operations.AddOperation
 import SP1Clean.ByteOpcodeTable
-import SP1Clean.GatedAddOp
+import SP1Clean.Operations.GatedAddOp
 import SP1Clean.ProgramTable
 import SP1Clean.MemoryAccess
 import SP1Clean.Reader.CPUState
