SP1Clean/LoadWordChip.lean
@@ -14,7 +14,7 @@ import SP1Operations.Reader.CPUState.CPUState
 import SP1Operations.Operation.U16MSBOperation.U16MSBOperation
 import SP1Operations.Operation.AddrAddOperation.AddrAddOperation
 import SP1Chips.Load.LoadWord.Common
-import SP1Clean.AddrAddOperation
+import SP1Clean.Operations.AddrAddOperation
 import SP1Clean.ByteOpcodeTable
 import SP1Clean.ProgramTable
 import SP1Clean.MemoryAccess
