SP1Clean/SubChip.lean
@@ -16,7 +16,7 @@ import SP1Chips.Sub.SubChip
 import SP1Chips.Sub.Common
 import SP1Chips.Soundness
 import SP1Clean.MemoryAccess
-import SP1Clean.SubOperation
+import SP1Clean.Operations.SubOperation
 import SP1Clean.ByteOpcodeTable
 import SP1Clean.ProgramTable
 import SP1Clean.Reader.CPUState
