SP1Operations/Reader/ALUTypeReader/Operation.lean
@@ -2,6 +2,7 @@ import SP1Foundations
 
 
 --- A Reader that only accesses values of type `T`.
+@[ext]
 structure ALUTypeReader (F : Type) where
   op_a : F
   op_a_memory : MemoryAccessInSharedCols F
